Datalog/Utils.lean
@@ -1,0 +1,7 @@
+def List.product (xs : List α) (len : Nat := 1) : List (List α) :=
+  match len with
+  | 0 => [[]]
+  | n + 1 => xs.product n |>.flatMap (fun p => xs.map (fun x => x :: p))
+
+#eval [1, 2, 3].product
+#eval [1, 2, 3].product 3
